continue
git-svn-id: https://projects.brucker.ch/hol-testgen/svn/HOL-TestGen/trunk/hol-testgen@12304 3260e6d1-4efc-4170-b0a7-36055960796d

examples/Flight_Model.thy
@@ -367,6 +367,9 @@ lemma F1_val_seatsATpre: "(\<sigma>\<^sub>s\<^sub>1, \<sigma>) \<Turnstile> F1 .
             qed
        qed
 
+lemma F1_val_seatsATpre': "\<sigma>\<^sub>s\<^sub>1 \<Turnstile>\<^sub>p\<^sub>r\<^sub>e F1 .seats@pre \<triangleq> \<guillemotleft>120\<guillemotright>"
+by(simp add: OclValid_at_pre_def F1_val_seatsATpre)
+
 lemma F2_val_seatsATpre: "(\<sigma>\<^sub>s\<^sub>1, \<sigma>) \<Turnstile> F2 .seats@pre \<triangleq> \<guillemotleft>370\<guillemotright>"
       proof(simp add: UML_Logic.foundation22 k_def )
          show "F2 .seats@pre (\<sigma>\<^sub>s\<^sub>1, \<sigma>) = \<lfloor>\<lfloor>370\<rfloor>\<rfloor>"
@@ -380,6 +383,8 @@ lemma F2_val_seatsATpre: "(\<sigma>\<^sub>s\<^sub>1, \<sigma>) \<Turnstile> F2 .
             qed
        qed
 
+lemma F2_val_seatsATpre': "\<sigma>\<^sub>s\<^sub>1 \<Turnstile>\<^sub>p\<^sub>r\<^sub>e F2 .seats@pre \<triangleq> \<guillemotleft>370\<guillemotright>"
+by(simp add: OclValid_at_pre_def F2_val_seatsATpre)
 
 lemma F1_val_seats: "(\<sigma>, \<sigma>\<^sub>s\<^sub>2) \<Turnstile> F1 .seats \<triangleq> \<guillemotleft>120\<guillemotright>"
 proof(simp add: UML_Logic.foundation22 k_def )
@@ -394,6 +399,9 @@ proof(simp add: UML_Logic.foundation22 k_def )
         qed
 qed
 
+lemma F1_val_seats': "\<sigma>\<^sub>s\<^sub>2 \<Turnstile>\<^sub>p\<^sub>o\<^sub>s\<^sub>t F1 .seats \<triangleq> \<guillemotleft>120\<guillemotright>"
+by(simp add: OclValid_at_post_def F1_val_seats)
+
 lemma F2_val_seats: "(\<sigma>, \<sigma>\<^sub>s\<^sub>2) \<Turnstile> F2 .seats \<triangleq> \<guillemotleft>370\<guillemotright>"
 proof(simp add: UML_Logic.foundation22 k_def )
    show   "F2 .seats (\<sigma>, \<sigma>\<^sub>s\<^sub>2) =  \<lfloor>\<lfloor>370\<rfloor>\<rfloor>"
@@ -406,6 +414,9 @@ proof(simp add: UML_Logic.foundation22 k_def )
               by(simp add: reconst_basetype_def)
         qed
 qed
+
+lemma F2_val_seats': "\<sigma>\<^sub>s\<^sub>2 \<Turnstile>\<^sub>p\<^sub>o\<^sub>s\<^sub>t F2 .seats \<triangleq> \<guillemotleft>370\<guillemotright>"
+by(simp add: OclValid_at_post_def F2_val_seats)
 
 lemma C1_valid: "(\<sigma>\<^sub>s\<^sub>1, \<sigma>') \<Turnstile> (\<upsilon> C1)"
 by(simp add: OclValid_def C1_def)
@@ -461,6 +472,12 @@ Context f: Flight
   Inv B : "f .fl_res ->size\<^sub>S\<^sub>e\<^sub>q() \<le>\<^sub>i\<^sub>n\<^sub>t (f .seats)"
   Inv C : "f .passengers ->select\<^sub>S\<^sub>e\<^sub>t(p | p .oclIsTypeOf(Client))
                           \<doteq> ((f .fl_res)->collect\<^sub>S\<^sub>e\<^sub>q(c | c .client .oclAsType(Person))->asSet\<^sub>S\<^sub>e\<^sub>q())"
+
+(* TODO : the following low-level properties should also 
+          be proven automatically. *)
+
+definition "Flight_A\<^sub>p\<^sub>r\<^sub>e = (\<lambda>\<sigma>. \<sigma> \<Turnstile>\<^sub>p\<^sub>r\<^sub>e Flight .allInstances@pre()->forAll\<^sub>S\<^sub>e\<^sub>t(self|Flight .allInstances@pre()->forAll\<^sub>S\<^sub>e\<^sub>t(f|\<zero> <\<^sub>i\<^sub>n\<^sub>t f .seats@pre)))"
+definition "Flight_A\<^sub>p\<^sub>o\<^sub>s\<^sub>t = (\<lambda>\<sigma>. \<sigma> \<Turnstile>\<^sub>p\<^sub>o\<^sub>s\<^sub>t Flight .allInstances()->forAll\<^sub>S\<^sub>e\<^sub>t(self|Flight .allInstances()->forAll\<^sub>S\<^sub>e\<^sub>t(f|\<zero> <\<^sub>i\<^sub>n\<^sub>t f .seats)))"
 
 (* This lemma would be highly desirable, but well ... *)
 lemma Flight_A_prepost_transfer: "Flight_Aat_pre (\<sigma>, \<sigma>') = Flight_A (\<sigma>'', \<sigma>)"
@@ -603,6 +620,9 @@ next
        qed
 qed
 
+lemma Flight_consistent': "(\<exists> \<sigma>\<^sub>p\<^sub>r\<^sub>e. Flight_A\<^sub>p\<^sub>r\<^sub>e \<sigma>\<^sub>p\<^sub>r\<^sub>e) \<and> (\<exists> \<sigma>\<^sub>p\<^sub>o\<^sub>s\<^sub>t. Flight_A\<^sub>p\<^sub>o\<^sub>s\<^sub>t \<sigma>\<^sub>p\<^sub>o\<^sub>s\<^sub>t)"
+oops
+
 Context r: Reservation
   Inv A : "\<zero> <\<^sub>i\<^sub>n\<^sub>t (r .id)"
   Inv B : "r .next <> null implies (r .flight .to \<doteq> r .next .flight .from)"
@@ -664,52 +684,58 @@ lemma cancel\<^sub>n\<^sub>o\<^sub>n\<^sub>b\<^sub>l\<^sub>o\<^sub>c\<^sub>k\<^s
 by(subst cp_valid, simp, subst cp_valid[symmetric],
    simp add: C1_valid[simplified OclValid_def \<sigma>\<^sub>t\<^sub>1_\<sigma>\<^sub>s\<^sub>1[symmetric]])
 
+lemma cancel\<^sub>n\<^sub>o\<^sub>n\<^sub>b\<^sub>l\<^sub>o\<^sub>c\<^sub>k\<^sub>i\<^sub>n\<^sub>g_\<^sub>p\<^sub>r\<^sub>e : "\<exists> self r \<sigma>.  \<sigma> \<Turnstile>\<^sub>p\<^sub>r\<^sub>e (cancel\<^sub>p\<^sub>r\<^sub>e  self r)"
+ apply(rule exI[where x = "C1"], rule exI[where x = "R11"], rule exI[where x = "\<sigma>\<^sub>t\<^sub>1"])
+ apply(simp add: OclValid_at_pre_def, intro allI)
+ proof - fix \<sigma>' show "(\<sigma>\<^sub>t\<^sub>1, \<sigma>') \<Turnstile> cancel\<^sub>p\<^sub>r\<^sub>e C1 R11"
+ using R11_val_clientATpre[simplified OclValid_def StrongEq_def true_def \<sigma>\<^sub>t\<^sub>1_\<sigma>\<^sub>s\<^sub>1[symmetric], of \<sigma>']
+  apply(simp add: cancel\<^sub>p\<^sub>r\<^sub>e_def StrictRefEq\<^sub>O\<^sub>b\<^sub>j\<^sub>e\<^sub>c\<^sub>t_\<^sub>R\<^sub>e\<^sub>s\<^sub>e\<^sub>r\<^sub>v\<^sub>a\<^sub>t\<^sub>i\<^sub>o\<^sub>n StrictRefEq\<^sub>O\<^sub>b\<^sub>j\<^sub>e\<^sub>c\<^sub>t_def OclValid_at_pre_def OclValid_def)
+ by(subst cp_valid, simp, subst cp_valid[symmetric],
+    simp add: C1_valid[simplified OclValid_def \<sigma>\<^sub>t\<^sub>1_\<sigma>\<^sub>s\<^sub>1[symmetric]])
+qed
+
 lemma cancel\<^sub>i\<^sub>m\<^sub>p\<^sub>l\<^sub>e\<^sub>m\<^sub>e\<^sub>n\<^sub>t\<^sub>a\<^sub>b\<^sub>l\<^sub>e :
- assumes self_defined: "\<And>\<sigma> \<sigma>'. (\<sigma>, \<sigma>') \<Turnstile> \<delta> self"  (* self must be defined; since self is an 
-                                              object representation (and not a reference)
-                                              the pre and post states are arbitrary *)
- assumes pre_satisfied:"\<And> \<sigma>'. (\<sigma>,\<sigma>') \<Turnstile> (cancel\<^sub>p\<^sub>r\<^sub>e  self r)"
- shows                 "\<exists> \<sigma>' result. ((\<sigma>,\<sigma>') \<Turnstile> (cancel\<^sub>p\<^sub>o\<^sub>s\<^sub>t  self r result))"
+(* assumes pre_satisfied: "\<sigma> \<Turnstile>\<^sub>p\<^sub>r\<^sub>e (cancel\<^sub>p\<^sub>r\<^sub>e  self r)"*)
+ shows                  "\<exists> \<sigma>' result. ((\<sigma>,\<sigma>') \<Turnstile> \<delta> self) \<longrightarrow>
+                                      ((\<sigma>,\<sigma>') \<Turnstile> \<upsilon> r) \<longrightarrow>
+                                      ((\<sigma>,\<sigma>') \<Turnstile> (cancel\<^sub>p\<^sub>o\<^sub>s\<^sub>t  self r result))"
 proof -
- def \<sigma>'' \<equiv> "\<lparr> heap = let oid_self = oid_of (self (\<sigma>\<^sub>0,\<sigma>\<^sub>0)) in
-                     Map.empty (oid_self \<mapsto> in\<^sub>C\<^sub>l\<^sub>i\<^sub>e\<^sub>n\<^sub>t (mk\<^sub>C\<^sub>l\<^sub>i\<^sub>e\<^sub>n\<^sub>t (mk\<E>\<X>\<T>\<^sub>C\<^sub>l\<^sub>i\<^sub>e\<^sub>n\<^sub>t oid_self None) None))
+ def \<sigma>'' \<equiv> "\<lparr> heap = K \<lfloor>in\<^sub>C\<^sub>l\<^sub>i\<^sub>e\<^sub>n\<^sub>t (mk\<^sub>C\<^sub>l\<^sub>i\<^sub>e\<^sub>n\<^sub>t (mk\<E>\<X>\<T>\<^sub>C\<^sub>l\<^sub>i\<^sub>e\<^sub>n\<^sub>t 0 None) None)\<rfloor>
             , assocs = Map.empty (oid\<^sub>C\<^sub>l\<^sub>i\<^sub>e\<^sub>n\<^sub>t_0___cl_res \<mapsto> []) \<rparr>"
 
- have self_defined': "(\<sigma>,\<sigma>'') \<Turnstile> \<delta> self"
- by(rule self_defined)
-
- have self_definition: "\<And> \<sigma> \<sigma>'. \<exists>ta xa x. self (\<sigma>, \<sigma>') = \<lfloor>\<lfloor>mk\<^sub>C\<^sub>l\<^sub>i\<^sub>e\<^sub>n\<^sub>t (mk\<E>\<X>\<T>\<^sub>C\<^sub>l\<^sub>i\<^sub>e\<^sub>n\<^sub>t ta xa) x\<rfloor>\<rfloor>"
-  apply(case_tac "self (\<sigma>, \<sigma>')",
-        simp add: self_defined[simplified foundation16'])
-  apply (metis bot_option_def foundation18' foundation20 self_defined)
-  apply(simp)
-  proof - fix \<sigma> \<sigma>' a show "self (\<sigma>, \<sigma>') = \<lfloor>a\<rfloor> \<Longrightarrow> \<exists>ta xa x. a = \<lfloor>mk\<^sub>C\<^sub>l\<^sub>i\<^sub>e\<^sub>n\<^sub>t (mk\<E>\<X>\<T>\<^sub>C\<^sub>l\<^sub>i\<^sub>e\<^sub>n\<^sub>t ta xa) x\<rfloor>"
-  apply(case_tac a)
-  apply (metis bot_option_def foundation16' null_fun_def null_option_def self_defined,simp)
-  proof - fix aa show " self (\<sigma>, \<sigma>') = \<lfloor>\<lfloor>aa\<rfloor>\<rfloor> \<Longrightarrow> \<exists>ta xa x. aa = mk\<^sub>C\<^sub>l\<^sub>i\<^sub>e\<^sub>n\<^sub>t (mk\<E>\<X>\<T>\<^sub>C\<^sub>l\<^sub>i\<^sub>e\<^sub>n\<^sub>t ta xa) x" 
+ have self_definition: "\<And>\<tau>. \<tau> \<Turnstile> \<delta> self \<Longrightarrow> \<exists>ta xa x. self \<tau> = \<lfloor>\<lfloor>mk\<^sub>C\<^sub>l\<^sub>i\<^sub>e\<^sub>n\<^sub>t (mk\<E>\<X>\<T>\<^sub>C\<^sub>l\<^sub>i\<^sub>e\<^sub>n\<^sub>t ta xa) x\<rfloor>\<rfloor>"
+  apply(simp add:OclValid_def defined_def true_def false_def split: split_if_asm)
+  proof - fix \<tau> show "self \<tau> \<noteq> \<bottom> \<tau> \<and> self \<tau> \<noteq> null \<tau> \<Longrightarrow>
+         \<exists>ta xa x. self \<tau> = \<lfloor>\<lfloor>mk\<^sub>C\<^sub>l\<^sub>i\<^sub>e\<^sub>n\<^sub>t (mk\<E>\<X>\<T>\<^sub>C\<^sub>l\<^sub>i\<^sub>e\<^sub>n\<^sub>t ta xa) x\<rfloor>\<rfloor>"
+  apply(case_tac "self \<tau>", simp add: bot_option_def bot_fun_def, simp)  
+  proof - fix a show "\<lfloor>a\<rfloor> \<noteq> \<bottom> \<tau> \<and> \<lfloor>a\<rfloor> \<noteq> null \<tau> \<Longrightarrow>
+         self \<tau> = \<lfloor>a\<rfloor> \<Longrightarrow> \<exists>ta xa x. a = \<lfloor>mk\<^sub>C\<^sub>l\<^sub>i\<^sub>e\<^sub>n\<^sub>t (mk\<E>\<X>\<T>\<^sub>C\<^sub>l\<^sub>i\<^sub>e\<^sub>n\<^sub>t ta xa) x\<rfloor>"
+  apply(case_tac "a", simp add: null_fun_def null_option_def bot_option_def, simp)
+  proof - fix aa show " \<lfloor>\<lfloor>aa\<rfloor>\<rfloor> \<noteq> \<bottom> \<tau> \<and> \<lfloor>\<lfloor>aa\<rfloor>\<rfloor> \<noteq> null \<tau> \<Longrightarrow>
+          self \<tau> = \<lfloor>\<lfloor>aa\<rfloor>\<rfloor> \<Longrightarrow>
+          a = \<lfloor>aa\<rfloor> \<Longrightarrow> \<exists>ta xa x. aa = mk\<^sub>C\<^sub>l\<^sub>i\<^sub>e\<^sub>n\<^sub>t (mk\<E>\<X>\<T>\<^sub>C\<^sub>l\<^sub>i\<^sub>e\<^sub>n\<^sub>t ta xa) x"
   apply(case_tac aa, simp)
-  proof - fix x1 x2 show " self (\<sigma>, \<sigma>') = \<lfloor>\<lfloor>mk\<^sub>C\<^sub>l\<^sub>i\<^sub>e\<^sub>n\<^sub>t x1 x2\<rfloor>\<rfloor> \<Longrightarrow> \<exists>ta xa. x1 = mk\<E>\<X>\<T>\<^sub>C\<^sub>l\<^sub>i\<^sub>e\<^sub>n\<^sub>t ta xa"
+  proof - fix x1 x2 show " self \<tau> = \<lfloor>\<lfloor>mk\<^sub>C\<^sub>l\<^sub>i\<^sub>e\<^sub>n\<^sub>t x1 x2\<rfloor>\<rfloor> \<Longrightarrow> \<exists>ta xa. x1 = mk\<E>\<X>\<T>\<^sub>C\<^sub>l\<^sub>i\<^sub>e\<^sub>n\<^sub>t ta xa"
   by(case_tac x1, simp)
-  qed qed qed 
+  qed qed qed qed 
 
- have self_empty: "(\<sigma>, \<sigma>'') \<Turnstile> (self .cl_res \<triangleq> Set{})"
+ have self_empty: "(\<sigma>, \<sigma>'') \<Turnstile> \<delta> self \<Longrightarrow> (\<sigma>, \<sigma>'') \<Turnstile> (self .cl_res \<triangleq> Set{})"
+  apply(drule self_definition, elim exE)
   apply(simp add: OclValid_def StrongEq_def dot\<^sub>C\<^sub>l\<^sub>i\<^sub>e\<^sub>n\<^sub>t_0___cl_res)
-  apply(insert self_definition[of \<sigma>\<^sub>0 \<sigma>\<^sub>0], elim exE)
-apply, elim exE, simp)
   apply(simp add: deref_oid\<^sub>C\<^sub>l\<^sub>i\<^sub>e\<^sub>n\<^sub>t_def in_post_state_def, subst (8) \<sigma>''_def)
-  apply(simp add: Let_def oid_of_option_def deref_assocs\<^sub>C\<^sub>l\<^sub>i\<^sub>e\<^sub>n\<^sub>t_0___cl_res_def deref_assocs_def)
+  apply(simp add: Let_def K_def oid_of_option_def deref_assocs\<^sub>C\<^sub>l\<^sub>i\<^sub>e\<^sub>n\<^sub>t_0___cl_res_def deref_assocs_def)
   apply(subst (3) \<sigma>''_def, simp add: select\<^sub>C\<^sub>l\<^sub>i\<^sub>e\<^sub>n\<^sub>t__cl_res_def)
   by(simp add: oid_of_ty\<^sub>C\<^sub>l\<^sub>i\<^sub>e\<^sub>n\<^sub>t_def deref_assocs_list_def switch\<^sub>2_01_def select_object\<^sub>S\<^sub>e\<^sub>t_def select_object_def)
 
  show "?thesis"
-  apply(rule exI[where x = \<sigma>''], rule exI[where x = "null"])
+  apply(rule exI[where x = \<sigma>''], rule exI[where x = "null"], intro impI)
   apply(simp add: cancel\<^sub>p\<^sub>o\<^sub>s\<^sub>t_def)
   apply(subst StrongEq_L_subst3[OF _ self_empty])
-   apply(rule UML_Set.cp_intro''\<^sub>S\<^sub>e\<^sub>t(2))
-   apply(simp only: cp_def)
-   apply(rule exI[where x = "\<lambda>X \<tau>. (\<lambda>_. X)->select\<^sub>S\<^sub>e\<^sub>t(res|StrictRefEq\<^sub>O\<^sub>b\<^sub>j\<^sub>e\<^sub>c\<^sub>t res .flight r .flight@pre) \<tau>"],
-         subst cp_OclSelect, simp)
- by(simp)
+    apply(rule UML_Set.cp_intro''\<^sub>S\<^sub>e\<^sub>t(2))
+    apply(simp only: cp_def)
+    apply(rule exI[where x = "\<lambda>X \<tau>. (\<lambda>_. X)->select\<^sub>S\<^sub>e\<^sub>t(res|StrictRefEq\<^sub>O\<^sub>b\<^sub>j\<^sub>e\<^sub>c\<^sub>t res .flight r .flight@pre) \<tau>"],
+          subst cp_OclSelect, simp)
+ by(simp+)
 qed
 
 find_theorems (350) name:"Client"
